src/cardinality/alk.lean
@@ -1,0 +1,127 @@
+/-
+The at-least-k boolean function.
+
+Authors: Cayden Codel, Jeremy Avigad, Marijn Heule
+Carnegie Mellon University
+-/
+
+import data.list.basic
+import cnf.literal
+import cnf.assignment
+import cnf.clause
+import cardinality.distinct
+import cardinality.amk
+
+variables {V : Type*} [decidable_eq V] [inhabited V]
+
+open assignment
+open clause
+open list
+open nat
+open distinct
+open amk
+
+def alk (k : nat) (l : list bool) : bool := l.count tt ≥ k
+
+namespace alk
+
+protected def eval (k : nat) (τ : assignment V) (l : list (literal V)) : bool :=
+  alk k (l.map (literal.eval τ))
+
+@[simp] theorem eval_zero : ∀ (τ : assignment V) (l : list (literal V)), 
+  alk.eval 0 τ l = tt :=
+assume τ l, by simp only [alk.eval, alk, ge_iff_le, zero_le, to_bool_true_eq_tt]
+
+@[simp] theorem eval_nil_ff_iff_pos {k : nat} :
+  ∀ τ, (alk.eval k τ ([] : list (literal V)) = ff ↔ k > 0) :=
+assume τ, by simp [alk.eval, alk, pos_iff_ne_zero]
+
+@[simp] theorem eval_nil_tt_iff_zero {k : nat} :
+  ∀ τ, (alk.eval k τ ([] : list (literal V)) = tt ↔ k = 0) :=
+assume τ, by simp [alk.eval, alk]
+
+variables {k : nat} {τ : assignment V} {lit : literal V} {l : list (literal V)}
+
+theorem eval_cons_pos : lit.eval τ = tt → 
+  ∀ l, alk.eval (k + 1) τ (lit :: l) = alk.eval k τ l :=
+assume hlit l, by simp [alk.eval, alk, hlit, succ_le_succ_iff]
+
+theorem eval_cons_neg : lit.eval τ = ff → 
+  ∀ l, alk.eval k τ (lit :: l) = alk.eval k τ l :=
+assume hlit l, by simp [alk.eval, alk, hlit]
+
+theorem eval_take_tail_pos {i : nat} (Hi : i < length l) : 
+  (l.nth_le i Hi).eval τ = tt → 
+  alk.eval (k + 1) τ (l.take (i + 1)) = alk.eval k τ (l.take i) :=
+begin
+  intro hl,
+  induction i with i ih generalizing l k,
+  { rw nth_le_zero at hl,
+    simp [take_one_of_ne_nil (ne_nil_of_length_pos Hi), hl, alk.eval, alk] },
+  { rcases exists_cons_of_ne_nil (ne_nil_of_length_pos (pos_of_gt Hi)) with ⟨l₁, ls, rfl⟩,
+    rw nth_le at hl,
+    cases h₁ : l₁.eval τ,
+    { simp only [take, eval_cons_neg h₁, ih (succ_lt_succ_iff.mp Hi) hl] },
+    { cases k,
+      { simp [alk.eval, alk, h₁, succ_le_succ_iff] },
+      { simp [take, eval_cons_pos h₁],
+        exact ih (succ_lt_succ_iff.mp Hi) hl } } }
+end
+
+theorem eval_take_tail_neg {i : nat} (Hi : i < length l) :
+  (l.nth_le i Hi).eval τ = ff →
+  alk.eval k τ (l.take (i + 1)) = alk.eval k τ (l.take i) :=
+begin
+  intro hl,
+  induction i with i ih generalizing l k,
+  { rw nth_le_zero at hl,
+    simp [take_one_of_ne_nil (ne_nil_of_length_pos Hi), hl, alk.eval, alk] },
+  { rcases exists_cons_of_ne_nil (ne_nil_of_length_pos (pos_of_gt Hi)) with ⟨l₁, ls, rfl⟩,
+    rw nth_le at hl,
+    cases h₁ : l₁.eval τ,
+    { simp [take, eval_cons_neg h₁, ih (succ_le_succ_iff.mp Hi) hl] },
+    { cases k,
+      { simp [take, alk.eval, alk] },
+      { simp [take, eval_cons_pos h₁,ih (succ_le_succ_iff.mp Hi) hl] } } }
+end
+
+theorem eval_tt_of_ge_of_eval_tt {k₁ k₂ : nat} : k₁ ≥ k₂ → 
+  alk.eval k₁ τ l = tt → alk.eval k₂ τ l = tt :=
+begin
+  simp only [alk.eval, alk, ge_iff_le, to_bool_iff],
+  intros hk h₁,
+  exact le_trans hk h₁
+end
+
+theorem eval_tt_of_sublist_of_eval_tt {l₁ l₂ : list (literal V)} :
+  l₁ <+ l₂ → alk.eval k τ l₁ = tt → alk.eval k τ l₂ = tt :=
+begin
+  simp [alk.eval, alk],
+  intros hls h₁,
+  exact le_trans h₁ (sublist.count_le (sublist.map (literal.eval τ) hls) tt)
+end
+
+theorem amk_alk_take {k : nat} {l : list (literal V)} {i : nat} :
+  i ≤ length l → ∀ (τ : assignment V), alk.eval k τ (l.take i) = tt →
+  amk.eval k τ l = tt → amk.eval 0 τ (l.drop i) = tt :=
+begin
+  intros hi τ htake hamk,
+  induction l with l₁ ls ih generalizing k i,
+  { simp only [drop_eq_nil_of_le, length, zero_le, amk.eval_nil] },
+  { cases i,
+    { simp at htake, subst htake,
+      rw drop,
+      exact hamk },
+    { cases k,
+      { exact eval_drop i.succ hamk },
+      { rw [length, succ_le_succ_iff] at hi,
+        cases hl₁ : (l₁.eval τ),
+        { rw [take, eval_cons_neg hl₁] at htake,
+          rw amk.eval_cons_neg hl₁ at hamk,
+          exact ih hi htake hamk },
+        { rw [take, eval_cons_pos hl₁] at htake,
+          rw amk.eval_cons_pos hl₁ at hamk,
+          exact ih hi htake hamk } } } }
+end
+
+end alk
