src/cardinality/amk.lean
@@ -1,0 +1,397 @@
+/-
+This file defines the at-most-k Boolean cardinality constraint.
+
+Authors: Cayden Codel, Jeremy Avigad, Marijn Heule
+Carnegie Mellon University
+-/
+
+import data.list.basic
+import cnf.literal
+import cnf.assignment
+import cnf.clause
+import cardinality.distinct
+
+variables {V : Type*} [decidable_eq V] [inhabited V]
+
+open assignment
+open clause
+open list
+open nat
+open distinct
+
+def amk (k : nat) (l : list bool) : bool := l.count tt ≤ k
+
+namespace amk
+
+/-
+theorem eval_tt_of_eval_tt_cons {τ : assignment V} {l : list (literal V)} 
+  {lit : literal V} : amz.eval τ (lit :: l) = tt → amz.eval τ l = tt :=
+begin
+  intro h,
+  rw eval_tt_iff_forall_eval_ff at h,
+  apply eval_tt_iff_forall_eval_ff.mpr,
+  intros lit hl,
+  exact h lit (mem_cons_of_mem _ hl)
+end
+
+theorem eval_cons_eq_of_eval_ff {τ : assignment V} {l : list (literal V)}
+  {lit : literal V} : lit.eval τ = ff → amz.eval τ (lit :: l) = amz.eval τ l :=
+begin
+  intro h,
+  simp only [amz.eval, amz, h, map, count_cons_of_ne, ne.def, not_false_iff]
+end
+
+theorem eval_sublist {τ : assignment V} {l₁ l₂ : list (literal V)} :
+  l₁ <+ l₂ → amz.eval τ l₂ = tt → amz.eval τ l₁ = tt :=
+begin
+  simp [amz.eval, amz],
+  intros hs hamz,
+  have := sublist.count_le (sublist.map (literal.eval τ) hs) tt,
+  simp [hamz] at this,
+  exact this
+end
+
+theorem eval_drop {τ : assignment V} {l : list (literal V)} : ∀ i, 
+  amz.eval τ l = tt → amz.eval τ (l.drop i) = tt :=
+assume i hamz, eval_sublist (drop_sublist i l) hamz
+
+-- Encoding of at-most-zero is a clause for each literal, negated
+def direct_amz (l : list (literal V)) : cnf V := l.map (λ x, [literal.flip x])
+
+theorem direct_amz_encodes_amz (l : list (literal V)) :
+  l ≠ [] → encodes amz (direct_amz l) l :=
+begin
+  rw direct_amz,
+  intros hnil τ,
+  rcases exists_mem_of_ne_nil l hnil with ⟨lit, hlit⟩,
+  split,
+  { intro h,
+    use τ,
+    split,
+    { rw cnf.eval_tt_iff_forall_clause_eval_tt,
+      intros c hc,
+      rcases mem_map.mp hc with ⟨lit₂, hlit₂, rfl⟩,
+      rw eval_singleton,
+      rw eval_flip,
+      simp only [amz, to_bool_iff] at h,
+      have := mt (mem_map.mpr) (not_mem_of_count_eq_zero h),
+      simp only [not_exists, eq_ff_eq_not_eq_tt, not_and] at this,
+      simp only [this lit₂ hlit₂, bool.bnot_false] },
+    { exact eqod.refl τ _ } },
+  { rintros ⟨σ, heval, heqod⟩,
+    rw cnf.eval_tt_iff_forall_clause_eval_tt at heval,
+    simp [amz],
+    simp at heval,
+    apply count_eq_zero_of_not_mem,
+    simp [mem_map],
+    intros lit₂ hlit₂,
+    have := mem_vars_of_mem hlit₂,
+    rw eval_eq_of_eqod_of_var_mem heqod this,
+    have := heval lit₂ hlit₂,
+    simpa [eval_flip] using this }
+end
+
+-- TODO: There's a way to get a direct proof
+theorem eval_eq_amz_of_eqod {τ₁ τ₂ : assignment V} {l : list (literal V)} :
+  (τ₁ ≡clause.vars l≡ τ₂) → amz.eval τ₁ l = amz.eval τ₂ l :=
+begin
+  intro heqod,
+  induction l with l ls ih,
+  { simp only [amz.eval_nil] },
+  { have : literal.eval τ₁ l = literal.eval τ₂ l,
+    { have := mem_vars_of_mem (mem_cons_self l ls),
+      exact eval_eq_of_eqod_of_var_mem heqod this },
+    cases h : (literal.eval τ₁ l),
+    { rw eval_cons_eq_of_eval_ff h,
+      rw this at h,
+      rw eval_cons_eq_of_eval_ff h,
+      exact ih (eqod_subset (vars_subset_of_vars_cons l ls) heqod) },
+    { rw eval_ff_iff_exists_eval_tt.mpr ⟨l, mem_cons_self l ls, h⟩,
+      rw this at h,
+      rw eval_ff_iff_exists_eval_tt.mpr ⟨l, mem_cons_self l ls, h⟩ } }
+end
+-/
+
+@[simp] theorem amk_nil (k : nat) : amk k [] = tt := rfl
+
+@[simp] theorem amk_singleton_pos (k : nat) (b : bool) : amk (k + 1) [b] = tt :=
+by { cases b; simp [amk, count_singleton'] }
+
+protected def eval (k : nat) (τ : assignment V) (l : list (literal V)) : bool :=
+  amk k (l.map (literal.eval τ))
+
+variables (k : nat) (τ : assignment V) (l : list (literal V)) (lit : literal V)
+
+@[simp] theorem eval_nil : amk.eval k τ [] = tt :=
+by simp only [amk.eval, amk, count_nil, to_bool_true_eq_tt, zero_le, map_nil]
+
+@[simp] theorem eval_singleton_pos : amk.eval (k + 1) τ [lit] = tt :=
+by { cases h : lit.eval τ; simp [amk.eval, amk, count_singleton', h] }
+
+@[simp] theorem eval_singleton_zero : 
+  (amk.eval 0 τ [lit] = tt) ↔ lit.eval τ = ff :=
+begin
+  cases h : (lit.eval τ),
+  { split,
+    { tautology },
+    { intro _, simp [amk.eval, amk, h] } },
+  { split,
+    { intro hamk,
+      simp [amk.eval, amk] at hamk,
+      have := not_mem_of_count_eq_zero hamk,
+      simp [h] at this,
+      exfalso, exact this },
+    { intro h, contradiction } }
+end
+
+theorem eval_tt_of_ge_length {k : nat} {l : list (literal V)} :
+  k ≥ length l → ∀ (τ : assignment V), amk.eval k τ l = tt :=
+begin
+  intros hk τ,
+  simp [amk.eval, amk],
+  have := count_le_length tt (map (literal.eval τ) l),
+  rw length_map at this,
+  exact le_trans this hk
+end
+
+theorem eval_cons_pos {k : nat} {τ : assignment V} {lit : literal V} : 
+  lit.eval τ = tt → ∀ l, amk.eval (k + 1) τ (lit :: l) = amk.eval k τ l :=
+assume hlit l, by simp [amk.eval, amk, hlit, succ_le_succ_iff]
+
+theorem eval_cons_neg {k : nat} {τ : assignment V} {lit : literal V} :
+  lit.eval τ = ff → ∀ l, amk.eval k τ (lit :: l) = amk.eval k τ l :=
+assume hlit l, by simp [amk.eval, amk, hlit]
+
+theorem eval_tt_of_le_of_eval_tt {τ : assignment V} {l : list (literal V)} 
+  {k₁ k₂ : nat} : k₁ ≤ k₂ → amk.eval k₁ τ l = tt → amk.eval k₂ τ l = tt :=
+begin
+  simp only [amk.eval, amk, ge_iff_le, to_bool_iff],
+  intros hk h₁,
+  exact le_trans h₁ hk  
+end
+
+theorem eval_sublist {k : nat} {τ : assignment V} {l₁ l₂ : list (literal V)} :
+  l₁ <+ l₂ → amk.eval k τ l₂ = tt → amk.eval k τ l₁ = tt :=
+begin
+  simp [amk.eval, amk],
+  intros hs h, 
+  exact le_trans (sublist.count_le (sublist.map (literal.eval τ) hs) tt) h
+end
+
+theorem eval_drop {k : nat} {τ : assignment V} {l : list (literal V)} :
+  amk.eval k τ l = tt → ∀ (i : nat), amk.eval k τ (l.drop i) = tt :=
+assume hamk i, eval_sublist (drop_sublist i l) hamk
+
+theorem eval_take {k : nat} {τ : assignment V} {l : list (literal V)} :
+  amk.eval k τ l = tt → ∀ (i : nat), amk.eval k τ (l.take i) = tt :=
+assume hamk i, eval_sublist (take_sublist i l) hamk 
+
+/-! # amz -/
+
+-- The special case where k = 0 is handled
+theorem amz_eval_tt_iff_forall_eval_ff :
+  amk.eval 0 τ l = tt ↔ (∀ (lit : literal V), lit ∈ l → lit.eval τ = ff) :=
+begin
+  split,
+  { simp [amk.eval, amk],
+    intro hc,
+    have := not_mem_of_count_eq_zero hc,
+    simp at this,
+    exact this },
+  { intro h,
+    rw [amk.eval, amk, to_bool_iff, le_zero_iff],
+    apply count_eq_zero_of_not_mem,
+    simpa }
+end
+
+-- Can be done with contrapose, somehow
+theorem amz_eval_ff_iff_exists_eval_tt :
+  amk.eval 0 τ l = ff ↔ (∃ (lit : literal V), lit ∈ l ∧ lit.eval τ = tt) :=
+begin
+  split,
+  { contrapose, simp,
+    exact (amz_eval_tt_iff_forall_eval_ff τ l).mpr },
+  { contrapose, simp,
+    exact (amz_eval_tt_iff_forall_eval_ff τ l).mp }
+end
+
+theorem eval_cons_pos_zero {τ : assignment V} {lit : literal V} :
+  lit.eval τ = tt → ∀ l, amk.eval 0 τ (lit :: l) = ff :=
+begin
+  intros hlit l,
+  apply (amz_eval_ff_iff_exists_eval_tt τ (lit :: l)).mpr,
+  use [lit, mem_cons_self _ _, hlit]
+end
+
+/-! # back to general theorems -/
+
+theorem eval_tail_pos {k i : nat} {τ : assignment V} {l : list (literal V)}
+  {hi : i < length l} : (l.nth_le i hi).eval τ = tt →
+  amk.eval (k + 1) τ (l.take (i + 1)) = amk.eval k τ (l.take i) :=
+begin
+  intro hamk,
+  induction l with l₁ ls ih generalizing i k,
+  { simp },
+  { cases i,
+    { simp },
+    { rw [take, take],
+      rw nth_le at hamk,
+      rw [length, succ_lt_succ_iff] at hi,
+      cases h₁ : (l₁.eval τ),
+      { rw [eval_cons_neg h₁, eval_cons_neg h₁],
+        exact ih hamk },
+      { cases k,
+        { rw eval_cons_pos_zero h₁, -- Can be tightened up
+          rw eval_cons_pos h₁,
+          by_contradiction,
+          rw [eq_tt_eq_not_eq_ff, amz_eval_tt_iff_forall_eval_ff] at h,
+          have : length (ls.take (i + 1)) = i + 1,
+          { have h := length_take (i + 1) ls,
+            have : min (i + 1) (length ls) = i + 1,
+            { simp [succ_le_of_lt hi] },
+            rw this at h,
+            exact h },
+          have hlen : i < length (ls.take (i + 1)),
+          { rw this,
+            exact lt_succ_self i },
+          have hmem := nth_le_mem _ _ hlen,
+          have : (ls.nth_le i _) = (ls.take (i.succ)).nth_le i hlen,
+          { rw this at hlen,
+            exact nth_le_take ls hi hlen },
+          rw ← this at hmem,
+          have hff := h _ hmem,
+          have : literal.eval τ (ls.nth_le i hi) = tt,
+          { assumption },
+          rw this at hff,
+          contradiction },
+        { rw [eval_cons_pos h₁, eval_cons_pos h₁],
+          exact ih hamk } } } }
+end
+
+theorem eval_tail_neg {k i : nat} {τ : assignment V} {l : list (literal V)}
+  {hi : i < length l} : (l.nth_le i hi).eval τ = ff →
+  amk.eval k τ (l.take (i + 1)) = amk.eval k τ (l.take i) :=
+begin
+  intro hamk,
+  induction l with l₁ ls ih generalizing i k,
+  { simp },
+  { cases i,
+    { simp at hamk, cases k; simp [hamk] },
+    { rw [take, take],
+      rw nth_le at hamk,
+      rw [length, succ_lt_succ_iff] at hi,
+      cases h₁ : (l₁.eval τ),
+      { rw [eval_cons_neg h₁, eval_cons_neg h₁],
+        exact ih hamk },
+      { cases k,
+        { rw [eval_cons_pos_zero h₁, eval_cons_pos_zero h₁] },
+        { rw [eval_cons_pos h₁, eval_cons_pos h₁],
+          exact ih hamk } } } }
+end
+
+-- Can probably be shortened with the correct order of cases
+theorem exists_amk_split {k : nat} {τ : assignment V} {l : list (literal V)} : 
+  amk.eval k τ l = tt → ∀ {k₁ k₂ : nat}, k₁ + k₂ = k → 
+  ∃ {l₁ l₂ : list (literal V)}, l₁ ++ l₂ = l ∧
+  amk.eval k₁ τ l₁ = tt ∧ amk.eval k₂ τ l₂ = tt :=
+begin
+  intros hamk k₁ k₂ hks,
+  induction l with lit₁ ls ih generalizing k k₁ k₂,
+  { use [[], []],
+    simp },
+  { cases k,
+    { cases hlit₁ : (literal.eval τ lit₁),
+      { rw eval_cons_neg hlit₁ at hamk,
+        rcases ih hamk hks with ⟨l₁, l₂, hls, hl₁, hl₂⟩,
+        use [(lit₁ :: l₁), l₂],
+        simp [hls, eval_cons_neg hlit₁, hl₁, hl₂] },
+      { rw [amz_eval_tt_iff_forall_eval_ff] at hamk,
+        rw (hamk _ (mem_cons_self lit₁ ls)) at hlit₁,
+        contradiction } },
+    { cases k₁,
+      { rw zero_add at hks, subst hks,
+        use [[], lit₁ :: ls],
+        simpa },
+      { cases hlit₁ : (literal.eval τ lit₁),
+        { rw eval_cons_neg hlit₁ at hamk,
+          rcases ih hamk hks with ⟨l₁, l₂, hls, hl₁, hl₂⟩,
+          use [(lit₁ :: l₁), l₂],
+          simp [hls, eval_cons_neg hlit₁, hl₁, hl₂] },
+        { rw succ_add at hks,
+          rw eval_cons_pos hlit₁ at hamk,
+          rcases ih hamk (succ.inj hks) with ⟨l₁, l₂, hls, hl₁, hl₂⟩,
+          use [(lit₁ :: l₁), l₂],
+          simp [hls, eval_cons_pos hlit₁, hl₁, hl₂] } } } }
+end
+
+theorem eval_eq_amk_of_eqod {τ₁ τ₂ : assignment V} {l : list (literal V)} :
+  ∀ (k : nat), (τ₁ ≡clause.vars l≡ τ₂) → amk.eval k τ₁ l = amk.eval k τ₂ l :=
+begin
+  intros k heqod,
+  induction l with l ls ih generalizing k,
+  { simp only [eval_nil] },
+  { have := eval_eq_of_eqod_of_var_mem heqod (mem_vars_of_mem (mem_cons_self l ls)),
+    cases h : (l.eval τ₁),
+    { rw eval_cons_neg h,
+      rw this at h,
+      rw eval_cons_neg h,
+      exact ih (eqod_subset (vars_subset_of_vars_cons _ _) heqod) k },
+    { cases k,
+      { rw eval_cons_pos_zero h,
+        rw this at h,
+        rw eval_cons_pos_zero h },
+      { rw eval_cons_pos h,
+        rw this at h,
+        rw eval_cons_pos h,
+        exact ih (eqod_subset (vars_subset_of_vars_cons _ _) heqod) k } } }
+end
+
+/-! # amo -/
+
+theorem amo_eval_tt_iff_distinct_eval_ff_of_eval_tt 
+  {τ : assignment V} {l : list (literal V)} :
+  amk.eval 1 τ l = tt ↔ (∀ {lit₁ lit₂ : literal V}, 
+  distinct lit₁ lit₂ l → lit₁.eval τ = tt → lit₂.eval τ = ff) :=
+begin
+  induction l with l₁ ls ih,
+  { split,
+    { intros _ lit₁ lit₂ hdis,
+      exact absurd hdis (not_distinct_nil _ _) },
+    { rw eval_nil, tautology } },
+  { cases ls with l₂ ls,
+    { split,
+      { intros _ lit₁ lit₂ hdis,
+        exact absurd hdis (not_distinct_singleton _ _ _) },
+      { rw eval_singleton_pos, tautology } },
+    { split,
+      { intros heval lit₁ lit₂ hdis h₁,
+        have hmem₂ := mem_tail_of_distinct_cons hdis,
+        rcases hdis with ⟨i, j, hi, hj, hij, hil, hjl⟩,
+        cases i,
+        { rw nth_le at hil,
+          rw [hil, eval_cons_pos h₁, amz_eval_tt_iff_forall_eval_ff] at heval,
+          exact heval lit₂ hmem₂ },
+        { cases j,
+          { linarith },
+          { have : distinct lit₁ lit₂ (l₂ :: ls),
+            { rw [length, succ_lt_succ_iff] at hi hj,
+              rw succ_lt_succ_iff at hij,
+              rw nth_le at hil hjl,
+              exact ⟨i, j, hi, hj, hij, hil, hjl⟩ },
+            cases h : (literal.eval τ l₁),
+            { rw eval_cons_neg h at heval,
+              exact ih.mp heval this h₁ },
+            { rw [eval_cons_pos h, amz_eval_tt_iff_forall_eval_ff] at heval,
+              exact heval lit₂ hmem₂ } } } },
+      { intro h,
+        cases h₁ : (literal.eval τ l₁),
+        { rw eval_cons_neg h₁,
+          apply ih.mpr,
+          intros lit₁ lit₂ hdis' h₁',
+          exact h (distinct_cons_of_distinct l₁ hdis') h₁' },
+        { rw [eval_cons_pos h₁, amz_eval_tt_iff_forall_eval_ff],
+          intros x hx,
+          exact h (distinct_cons_of_mem l₁ hx) h₁ } } } }
+end
+
+end amk
