src/cardinality/direct_amo.lean
@@ -1,0 +1,282 @@
+/-
+The direct encoding for the at-most-one function.
+
+Authors: Cayden Codel, Jeremy Avigad, Marijn Heule
+Carnegie Mellon University
+-/
+
+import cnf.literal
+import cnf.assignment
+import cnf.clause
+import cnf.cnf
+import cnf.encoding
+
+import cardinality.amk
+import cardinality.distinct
+
+variables {V : Type*} [decidable_eq V] [inhabited V]
+
+open list
+open nat
+open amk
+open clause
+open assignment
+open literal
+open cnf
+open distinct
+open encoding
+
+namespace direct_amo
+
+def direct_amo : list (literal V) → cnf V
+| []        := []
+| (l :: ls) := (ls.map (λ m, [l.flip, m.flip])) ++ (direct_amo ls)
+
+@[simp] theorem direct_amo_nil : direct_amo ([] : list (literal V)) = [] := rfl
+
+@[simp] theorem direct_amo_singleton (lit : literal V) : 
+  direct_amo [lit] = [] := rfl
+
+@[simp] theorem direct_amo_double (l₁ l₂ : literal V) :
+  direct_amo [l₁, l₂] = [[l₁.flip, l₂.flip]] := rfl
+
+theorem exists_mem_of_length_ge_two :
+  ∀ {l : list (literal V)}, length l ≥ 2 → ∃ (c : clause V), c ∈ direct_amo l
+| []   hl := by { rw length at hl, linarith }
+| [l₁] hl := by { rw [length, length] at hl, linarith }
+| (l₁ :: l₂ :: ls) hl := begin
+  use [[l₁.flip, l₂.flip]],
+  rw [direct_amo, mem_append], left,
+  simp only [map, mem_cons_iff, eq_self_iff_true, true_or]
+end
+
+theorem length_eq_two_of_mem {l : list (literal V)} {c : clause V} (hl : length l ≥ 2) :
+  c ∈ direct_amo l → length c = 2 :=
+begin
+  induction l with l₁ ls ih,
+  { rw length at hl, linarith },
+  { rw direct_amo,
+    simp only [mem_map, mem_append],
+    by_cases hls : length ls = 1,
+    { rcases exists_of_length_succ ls hls with ⟨l₂, ls, rfl⟩,
+      simp [length_eq_zero] at hls,
+      simp [hls],
+      rintro rfl,
+      dec_trivial },
+    { rw length at hl,
+      have := succ_le_succ_iff.mp hl,
+      have : 1 < ls.length, exact (ne.symm hls).le_iff_lt.mp this,
+      have : 2 ≤ ls.length, exact succ_le_iff.mpr this,
+      rintros (⟨a, ha, rfl⟩ | h),
+      { dec_trivial },
+      { exact ih this h } } }
+end
+
+-- TODO rename, distinct isn't used here
+theorem exists_double_flip_eq_of_mem {l : list (literal V)} {c : clause V} (hl : length l ≥ 2) :
+  c ∈ direct_amo l → ∃ (lit₁ lit₂ : literal V), [lit₁.flip, lit₂.flip] = c :=
+begin
+  intro h,
+  rcases exists_cons_cons_of_length_eq_two (length_eq_two_of_mem hl h) with ⟨lit₁, lit₂, rfl⟩,
+  use [lit₁.flip, lit₂.flip],
+  rw [flip_flip, flip_flip]
+end
+
+-- TODO this feels like a very long proof, can probably be shortened
+theorem distinct_iff_mem {l : list (literal V)} {lit₁ lit₂ : literal V} :
+  distinct lit₁ lit₂ l ↔ [lit₁.flip, lit₂.flip] ∈ direct_amo l :=
+begin
+  split,
+  { induction l with l₁ ls ih,
+    { intro h, exact absurd h (not_distinct_nil _ _) },
+    { intro h,
+      have hdis := h,
+      have hl := length_ge_two_of_distinct h,
+      rcases exists_cons_cons_of_length_ge_two hl with ⟨a₁, a₂, L, hL⟩,
+      rw ← (tail_eq_of_cons_eq hL) at *,
+      rw [direct_amo, mem_append],
+      rcases h with ⟨i, j, hi, hj, hij, hil, hjl⟩,
+      cases i,
+      { rw nth_le at hil,
+        left,
+        rw [hil, mem_map],
+        use [lit₂, mem_tail_of_distinct_cons hdis] },
+      { have : distinct lit₁ lit₂ (a₂ :: L),
+        { rw length at hi,
+          have := succ_le_iff.mpr ((gt_of_gt_of_ge hij (zero_le i.succ))),
+          rcases nth_le_of_ge hj this with ⟨h₁, h₂⟩,
+          rw length at h₁,
+          rw distinct,
+          use [i, j - 1, succ_lt_succ_iff.mp hi, succ_lt_succ_iff.mp h₁],
+          split,
+          { rw ← nat.sub_add_cancel this at hij,
+            exact succ_lt_succ_iff.mp hij },
+          rw nth_le at hil,
+          rw [hjl, nth_le] at h₂,
+          exact ⟨hil, h₂.symm⟩ },
+        exact or.inr (ih this) } } },
+  { induction l with l₁ ls ih,
+    { simp only [direct_amo_nil, not_mem_nil, forall_false_left] },
+    { cases ls with l₂ ls,
+      { rw direct_amo_singleton, intro h, exact absurd h (not_mem_nil _) },
+      cases ls with l₃ ls,
+      { rw [direct_amo_double, mem_singleton],
+        simp only [eq_self_iff_true, and_true, and_imp],
+        intros h₁ h₂,
+        rw [flip_inj.mp h₁, flip_inj.mp h₂],
+        use [0, 1], simp },
+      { intro h, -- TODO this feels very casewise
+        rw [direct_amo, mem_append] at h,
+        rcases h with (h | h),
+        { simp at h,
+          rcases h with (⟨h₁, h₂⟩ | ⟨h₁, h₃⟩ | ⟨l₄, hl₄, h₁, hls⟩),
+          { rw [flip_inj.mp h₁, flip_inj.mp h₂],
+            use [0, 1], simp },
+          { rw [flip_inj.mp h₁, flip_inj.mp h₃],
+            use [0, 2], simp, linarith }, -- can be done explicitly rather than linarith
+          { rw [flip_inj.mp h₁, ← flip_inj.mp hls],
+            rcases nth_le_of_mem hl₄ with ⟨n, hn, hln₄⟩,
+            use [0, n + 3],
+            simp,
+            use [succ_lt_succ (succ_lt_succ (succ_lt_succ hn)), hln₄] } },
+        { have : (l₂ :: l₃ :: ls).length ≥ 2,
+          { rw [length, length], linarith },
+          exact distinct_cons_of_distinct l₁ (ih h) } } } }
+end
+
+theorem subset_direct_of_sublist {l₁ l₂ : list (literal V)} :
+  l₁ <+ l₂ → (direct_amo l₁) ⊆ (direct_amo l₂) :=
+begin
+  induction l₂ with lit₁ ls ih generalizing l₁,
+  { rw sublist_nil_iff_eq_nil, rintro rfl, exact subset.refl _ },
+  { intros hl₁ c hc,
+    cases hl₁,
+    { rw [direct_amo, mem_append],
+      exact or.inr ((ih hl₁_ᾰ) hc) },
+    { rw [direct_amo, mem_append] at hc,
+      rcases hc with (hc | hc),
+      { rw mem_map at hc,
+        rcases hc with ⟨a, hal, hac⟩,
+        rw [direct_amo, mem_append, mem_map],
+        exact or.inl ⟨a, sublist.subset hl₁_ᾰ hal, hac⟩ },
+      { rw [direct_amo, mem_append],
+        exact or.inr (ih hl₁_ᾰ hc) } } }
+end
+
+theorem eval_tt_iff_forall_distinct_eval_ff {τ : assignment V} 
+  {l : list (literal V)} : length l ≥ 2 → ((direct_amo l).eval τ = tt ↔ 
+   (∀ {lit₁ lit₂ : literal V}, (distinct lit₁ lit₂ l) → lit₁.eval τ = ff ∨ lit₂.eval τ = ff)) :=
+begin
+  intro hl,
+  split,
+  { intros heval lit₁ lit₂ hdis,
+    rw cnf.eval_tt_iff_forall_clause_eval_tt at heval,
+    have := heval [lit₁.flip, lit₂.flip] (distinct_iff_mem.mp hdis),
+    rw eval_tt_iff_exists_literal_eval_tt at this,
+    rcases this with ⟨lit, hmem, hlit⟩,
+    simp only [mem_cons_iff, mem_singleton] at hmem,
+    rcases hmem with (rfl | rfl),
+    { rw eval_flip at hlit,
+      exact or.inl (bool.eq_ff_of_bnot_eq_tt hlit) },
+    { rw eval_flip at hlit,
+      exact or.inr (bool.eq_ff_of_bnot_eq_tt hlit) } },
+  { intro h,
+    rw cnf.eval_tt_iff_forall_clause_eval_tt,
+    intros c hc,
+    rcases exists_double_flip_eq_of_mem hl hc with ⟨l₁, l₂, rfl⟩,
+    have := h (distinct_iff_mem.mpr hc),
+    rw eval_tt_iff_exists_literal_eval_tt,
+    rcases h (distinct_iff_mem.mpr hc) with (hff | hff),
+    { use l₁.flip,
+      simp [eval_flip_of_eval hff] },
+    { use l₂.flip,
+      simp [eval_flip_of_eval hff] } }
+end
+
+theorem eval_tt_iff_forall_distinct_eval_ff_of_eval_tt {τ : assignment V} 
+  {l : list (literal V)} : length l ≥ 2 → ((direct_amo l).eval τ = tt ↔ 
+   (∀ {lit₁ lit₂ : literal V}, (distinct lit₁ lit₂ l) → lit₁.eval τ = tt → lit₂.eval τ = ff)) :=
+begin
+  intro hl,
+  split,
+  { intros ht lit₁ lit₂ hdis hlit₁, 
+    rcases (eval_tt_iff_forall_distinct_eval_ff hl).mp ht hdis with (h | h),
+    { rw h at hlit₁, contradiction },
+    { exact h } },
+  { intro hls,
+    apply (eval_tt_iff_forall_distinct_eval_ff hl).mpr,
+    intros lit₁ lit₂ hdis,
+    cases h : (literal.eval τ lit₁),
+    { exact or.inl (refl ff) },
+    { exact or.inr (hls hdis h) } }
+end
+
+theorem eval_ff_iff_forall_distinct_eval_tt {τ : assignment V}
+  {l : list (literal V)} (hl : length l ≥ 2) :
+  ((direct_amo l).eval τ = ff ↔ 
+  (∃ {lit₁ lit₂ : literal V}, (distinct lit₁ lit₂ l) ∧ lit₁.eval τ = tt ∧ lit₂.eval τ = tt)) :=
+begin
+  split,
+  { rw cnf.eval_ff_iff_exists_clause_eval_ff,
+    rintros ⟨c, hmem, hc⟩,
+    rcases exists_double_flip_eq_of_mem hl hmem with ⟨lit₁, lit₂, rfl⟩,
+    rw eval_ff_iff_forall_literal_eval_ff at hc,
+    use [lit₁, lit₂, distinct_iff_mem.mpr hmem],
+    have h₁ : lit₁.flip ∈ [lit₁.flip, lit₂.flip], from mem_cons_self _ _,
+    have h₂ : lit₂.flip ∈ [lit₁.flip, lit₂.flip], simp,
+    have h₁eval := eval_flip_of_eval (hc lit₁.flip h₁),
+    have h₂eval := eval_flip_of_eval (hc lit₂.flip h₂),
+    rw flip_flip at h₁eval h₂eval,
+    exact ⟨h₁eval, h₂eval⟩ },
+  { rintro ⟨lit₁, lit₂, hdis, h₁, h₂⟩,
+    rw cnf.eval_ff_iff_exists_clause_eval_ff,
+    use [[lit₁.flip, lit₂.flip], distinct_iff_mem.mp hdis],
+    rw eval_ff_iff_forall_literal_eval_ff,
+    simp [h₁, h₂, eval_flip] }
+end
+
+theorem direct_amo_encodes_amo : ∀ (l : list (literal V)),
+  encodes (amk 1) (direct_amo l) l
+| []   := by { intro τ, simp, }
+| [l₁] := by { intro τ, simp [← amk.eval], use τ }
+| (l₁ :: l₂ :: ls) := begin
+  have hl : length (l₁ :: l₂ :: ls) ≥ 2, dec_trivial,
+  intro τ, split,
+  { intro hamk, rw ← amk.eval at hamk,
+    rw amo_eval_tt_iff_distinct_eval_ff_of_eval_tt at hamk,
+    use τ,
+    split,
+    { rw cnf.eval_tt_iff_forall_clause_eval_tt,
+      intros c hc,
+      rw eval_tt_iff_exists_literal_eval_tt,
+      rcases exists_double_flip_eq_of_mem hl hc with ⟨lit₁, lit₂, rfl⟩,
+      cases h : (lit₁.eval τ),
+      { use [lit₁.flip, mem_cons_self _ _],
+        rw eval_flip,
+        simp only [h, bool.bnot_false] },
+      { have : lit₂.flip ∈ [lit₁.flip, lit₂.flip], simp,
+        use [lit₂.flip, this],
+        exact eval_flip_of_eval (hamk (distinct_iff_mem.mpr hc) h) } },
+    { exact eqod.refl _ _ } },
+  { rintros ⟨σ, heval, hsigma⟩,
+    rw cnf.eval_tt_iff_forall_clause_eval_tt at heval,
+    rw ← amk.eval,
+    rw amo_eval_tt_iff_distinct_eval_ff_of_eval_tt,
+    intros lit₁ lit₂ hdis h₁,
+    have := heval _ (distinct_iff_mem.mp hdis),
+    rw eval_tt_iff_exists_literal_eval_tt at this,
+    rcases this with ⟨lit, hmem, hlit⟩,
+    simp at hmem,
+    rcases hmem with (rfl | rfl),
+    { have := mem_vars_of_mem (mem_of_distinct_left hdis),
+      rw eval_eq_of_eqod_of_var_mem hsigma this at h₁,
+      rw [eval_flip, h₁] at hlit,
+      contradiction },
+    { have := mem_vars_of_mem (mem_of_distinct_right hdis),
+      have h₂ := eval_flip_of_eval hlit,
+      rw flip_flip at h₂,
+      rw ← eval_eq_of_eqod_of_var_mem hsigma this at h₂,
+      exact h₂ } }
+end
+
+end direct_amo
